src/extensions/paths/Replacement.v
@@ -17,6 +17,7 @@ Hint Constructors star.
 (** The following lemmas reason about the relationship between path
     replacement and the number of paths in a type *)
 
+(*
 Lemma repl_numpaths_relation_mutind:
   (forall n p q T U,
     repl_typ n p q T U ->
@@ -77,22 +78,22 @@ Lemma numpaths_open:
 Proof.
   apply typ_mutind; intros; simpl; eauto.
 Qed.
-
+**)
 (** If [T[q/p,n] = U] then [U[p/q,n] = T] *)
 Lemma repl_swap:
-  (forall n p q T T',
-      repl_typ n p q T T' ->
-      repl_typ n q p T' T) /\
-  (forall n p q D D',
-      repl_dec n p q D D' ->
-      repl_dec n q p D' D).
+  (forall p q T T',
+      repl_typ p q T T' ->
+      repl_typ q p T' T) /\
+  (forall p q D D',
+      repl_dec p q D D' ->
+      repl_dec q p D' D).
 Proof.
   apply repl_mutind; intros; eauto.
 Qed.
 
 (** Replacing the whole path of a singleton type *)
 Lemma repl_intro_sngl: forall p q,
-    repl_typ 0 p q {{ p }} {{ q }}.
+    repl_typ p q {{ p }} {{ q }}.
 Proof.
   intros p q.
   replace {{ p }} with {{ p •• nil }}.
@@ -105,22 +106,22 @@ Qed.
 (** As long as named paths are replaced with named paths, opening
     preserves the replacement relationship between types and declarations *)
 Lemma repl_open_rec:
-  (forall m p q T T',
-      repl_typ m p q T T' -> forall r n,
+  (forall p q T T',
+      repl_typ p q T T' -> forall n r,
       named_path p ->
       named_path q ->
-      repl_typ m p q (open_rec_typ_p n r T) (open_rec_typ_p n r T')) /\
-  (forall m p q D D',
-      repl_dec m p q D D' -> forall r n,
+      repl_typ p q (open_rec_typ_p n r T) (open_rec_typ_p n r T')) /\
+  (forall p q D D',
+      repl_dec p q D D' -> forall r n,
       named_path p ->
       named_path q ->
-      repl_dec m p q (open_rec_dec_p n r D) (open_rec_dec_p n r D')).
+      repl_dec p q (open_rec_dec_p n r D) (open_rec_dec_p n r D')).
 Proof.
   apply repl_mutind; intros;
-    try solve [unfolds open_typ_p, open_dec_p; simpls; eauto];
-    try solve [simpl; assert (numpaths U = numpaths (open_rec_typ_p n0 r0 U))
+    try solve [unfolds open_typ_p, open_dec_p; simpls; eauto].
+    (**try solve [simpl; assert (numpaths U = numpaths (open_rec_typ_p n0 r0 U))
                  as Hn by apply* numpaths_open;
-               rewrite* Hn].
+               rewrite* Hn].**)
   - Case "rpath"%string.
     simpl. repeat rewrite field_sel_open. repeat rewrite open_named_path; auto.
   - Case "rsngl"%string.
@@ -128,31 +129,33 @@ Proof.
 Qed.
 
 (** ...for types only *)
-Lemma repl_open: forall p q T T' r n,
-    repl_typ n p q T T' ->
+Lemma repl_open: forall p q T T' r,
+    repl_typ p q T T' ->
     named_path p ->
     named_path q ->
-    repl_typ n p q (open_typ_p r T) (open_typ_p r T').
+    repl_typ p q (open_typ_p r T) (open_typ_p r T').
 Proof.
   unfold open_typ_p. intros. apply* repl_open_rec.
 Qed.
 
 (** ... for opening with variables only*)
-Lemma repl_open_var: forall n p q T T' x,
-    repl_typ n p q T T' ->
+Lemma repl_open_var: forall p q T T' x,
+    repl_typ p q T T' ->
     named_path p ->
     named_path q ->
-    repl_typ n p q (open_typ x T) (open_typ x T').
+    repl_typ p q (open_typ x T) (open_typ x T').
 Proof.
   introv Hr. repeat rewrite open_var_typ_eq. apply* repl_open.
 Qed.
 
 (** Equivalent types (up to one replacement) *)
+(**
 Definition repl_some_typ p q T T' := exists n, repl_typ n p q T T'.
 Definition repl_some_dec p q D D' := exists n, repl_dec n p q D D'.
+**)
 (** Equivalent types (multiple replacements) *)
-Notation repl_repeat_typ p q := (star (repl_some_typ p q)).
-Notation repl_repeat_dec p q := (star (repl_some_dec p q)).
+Notation repl_repeat_typ p q := (star (repl_typ p q)).
+Notation repl_repeat_dec p q := (star (repl_dec p q)).
 
 (** The following lemmas construct equivalent types out of simpler equivalent types*)
 
@@ -161,11 +164,9 @@ Lemma repl_star_rcd: forall p q d1 d2,
   repl_repeat_dec p q d1 d2 ->
   repl_repeat_typ p q (typ_rcd d1) (typ_rcd d2).
 Proof.
-  introv Hs. dependent induction Hs.
+  introv Hs. dependent induction Hs. 
   apply star_refl. eapply star_trans. apply star_one.
-  unfolds repl_some_dec.
-  destruct_all. repeat eexists. constructor*.
-  eauto.
+  constructor*. eauto.
 Qed.
 
 Ltac solve_repl_star :=
@@ -174,12 +175,13 @@ Ltac solve_repl_star :=
   | [ H : repl_repeat_typ _ _ _ _ |- _ ] =>
     dependent induction H
   end;
-  eauto;
+  eauto.
+(**;
   match goal with
   | [ IH : (repl_repeat_typ _ _) ?T _ |- _ ] =>
     apply star_trans with (b:=T)
   end;
-  [apply star_one; unfolds repl_some_typ; destruct_all; repeat eexists; constructor* |]; eauto.
+  [apply star_one; constructor* |]; eauto.**)
 
 (** ...and intersecting equivalent types yields equivalent types *)
 Lemma repl_star_and1: forall T1 T2 U p q,
@@ -223,9 +225,7 @@ Lemma repl_star_typ1: forall T1 T2 U A p q,
 Proof.
   introv Hs. dependent induction Hs.
   apply star_refl. eapply star_trans. apply star_one.
-  unfolds repl_some_typ.
-  destruct_all. repeat eexists. constructor*.
-  eauto.
+  constructor*. eauto.
 Qed.
 
 Lemma repl_star_typ2: forall T1 T2 U A p q,
@@ -234,9 +234,7 @@ Lemma repl_star_typ2: forall T1 T2 U A p q,
 Proof.
   introv Hs. dependent induction Hs.
   apply star_refl. apply star_trans with (b:={A >: U <: b}). apply star_one.
-  unfolds repl_some_typ.
-  destruct_all. repeat eexists. constructor*.
-  eauto.
+  constructor*. eauto.
 Qed.
 
 Lemma repl_star_trm: forall T1 T2 a p q,
@@ -245,9 +243,7 @@ Lemma repl_star_trm: forall T1 T2 a p q,
 Proof.
   introv Hs. dependent induction Hs.
   apply star_refl. eapply star_trans. apply star_one.
-  unfolds repl_some_typ.
-  destruct_all. repeat eexists. constructor*.
-  eauto.
+  constructor*. eauto.
 Qed.
 
 (** Opening a type (or declaration) with different paths yields two equivalent types (or declarations) *)
@@ -264,14 +260,14 @@ Proof.
     apply* repl_star_and1.
     apply* repl_star_and2.
   - destruct p as [[pn | px] pbs]; destruct p0 as [p0x p0bs]; simpl.
-    case_if; destruct q as [qx qbs]; subst. apply star_one. eexists.
+    case_if; destruct q as [qx qbs]; subst. apply star_one. 
     repeat rewrite proj_rewrite_mult. eauto.
     apply star_refl.
     destruct q as [qx qbs]. apply star_refl.
   - apply* repl_star_bnd.
   - eapply star_trans. apply repl_star_all1. apply* H. apply repl_star_all2. apply* H0.
   - destruct p as [[pn | px] pbs]; destruct p0 as [p0x p0bs]; simpl.
-    case_if; destruct q as [qx qbs]; subst. apply star_one. eexists.
+    case_if; destruct q as [qx qbs]; subst. apply star_one. 
     repeat rewrite proj_rewrite_mult. eauto.
     apply star_refl.
     destruct q as [qx qbs]. apply star_refl.
@@ -289,48 +285,48 @@ Qed.
 (** Further properties of path replacement *)
 
 Lemma repl_insert_mutind:
-  (forall n p q T U,
-      repl_typ n p q T U ->
-      forall r, exists V, repl_typ n p r T V /\ repl_typ n r q V U) /\
-  (forall n p q T U,
-      repl_dec n p q T U ->
-      forall r, exists V, repl_dec n p r T V /\ repl_dec n r q V U).
+  (forall p q T U,
+      repl_typ p q T U ->
+      forall r, exists V, repl_typ p r T V /\ repl_typ r q V U) /\
+  (forall p q T U,
+      repl_dec p q T U ->
+      forall r, exists V, repl_dec p r T V /\ repl_dec r q V U).
 Proof.
   apply repl_mutind; intros;
   try (destruct (H r0) as [v [H0 H1]]); eauto.
 Qed.
 
-Lemma repl_insert: forall n p q T U r,
-    repl_typ n p q T U ->
-    exists V, repl_typ n p r T V /\ repl_typ n r q V U.
+Lemma repl_insert: forall p q T U r,
+    repl_typ p q T U ->
+    exists V, repl_typ p r T V /\ repl_typ r q V U.
 Proof.
   destruct repl_insert_mutind. eauto.
 Qed.
 
 Lemma repl_field_elim_mutind:
-  (forall n p q T U,
-      repl_typ n p q T U ->
+  (forall p q T U,
+      repl_typ p q T U ->
       forall p0 q0 a,
       p = p0•a -> q = q0•a ->
-      repl_typ n p0 q0 T U) /\
-  (forall n p q T U,
-      repl_dec n p q T U ->
+      repl_typ p0 q0 T U) /\
+  (forall p q T U,
+      repl_dec p q T U ->
       forall p0 q0 a,
       p = p0•a -> q = q0•a ->
-      repl_dec n p0 q0 T U).
+      repl_dec p0 q0 T U).
 Proof.
   apply repl_mutind; intros; subst;
   try (subst; repeat (rewrite sel_field_to_fields));
   eauto.
 Qed.
 
-Lemma repl_field_elim : forall n p q a T U,
-    repl_typ n p•a q•a T U ->
-    repl_typ n p q T U.
+Lemma repl_field_elim : forall p q a T U,
+    repl_typ p•a q•a T U ->
+    repl_typ p q T U.
 Proof.
   destruct repl_field_elim_mutind. eauto.
 Qed.
-
+(**
 Lemma repl_unique_mutind:
   (forall n p q T T1,
       repl_typ n p q T T1 ->
@@ -510,21 +506,21 @@ Lemma repl_preserved2 : forall n p q T U1 U2 m r s,
 Proof.
   destruct repl_preserved2_mutind; eauto.
 Qed.
-
-Lemma repl_prefixes_sngl: forall n p q p' q',
-    repl_typ n p q {{ p' }} {{ q' }} ->
+**)
+Lemma repl_prefixes_sngl: forall p q p' q',
+    repl_typ p q {{ p' }} {{ q' }} ->
     exists bs, p' = p •• bs /\ q' = q •• bs.
 Proof.
   introv Hr. inversions Hr. eauto.
 Qed.
 
-Lemma repl_prefixes_sel: forall n p q p' q' A,
-    repl_typ n p q (p' ↓ A) (q' ↓ A) ->
+Lemma repl_prefixes_sel: forall p q p' q' A,
+    repl_typ p q (p' ↓ A) (q' ↓ A) ->
     exists bs, p' = p •• bs /\ q' = q •• bs.
 Proof.
   introv Hr. inversions Hr. eauto.
 Qed.
-
+(**
 Lemma repl_prefixes_mutind:
   (forall n q1 p1 T T1,
       repl_typ n q1 p1 T T1 ->
@@ -562,7 +558,7 @@ Lemma repl_prefixes: forall n q1 p1 q2 p2 T T1 T2,
 Proof.
   destruct repl_prefixes_mutind; eauto.
 Qed.
-
+**)
 Lemma sel_fieldss_subst: forall x y p ds,
   subst_path x y p •• ds = (subst_path x y p) •• ds.
 Proof.
@@ -571,29 +567,26 @@ Proof.
 Qed.
 
 Lemma repl_typ_subst_mutind:
-  (forall n p q T U,
-    repl_typ n p q T U ->
+  (forall p q T U,
+    repl_typ p q T U ->
     forall x y,
-    repl_typ n (subst_path x y p) (subst_path x y q) (subst_typ x y T) (subst_typ x y U)) /\
-  (forall n p q T U,
-    repl_dec n p q T U ->
+    repl_typ (subst_path x y p) (subst_path x y q) (subst_typ x y T) (subst_typ x y U)) /\
+  (forall p q T U,
+    repl_dec p q T U ->
     forall x y,
-    repl_dec n (subst_path x y p) (subst_path x y q) (subst_dec x y T) (subst_dec x y U)).
+    repl_dec (subst_path x y p) (subst_path x y q) (subst_dec x y T) (subst_dec x y U)).
 Proof.
   apply repl_mutind; intros; simpl; try (constructor); eauto.
-  - erewrite <- numpaths_subst_typ. eapply rand2. eauto.
   - rewrite* sel_fieldss_subst.
     rewrite* sel_fieldss_subst.
-  - erewrite <- numpaths_subst_typ. eauto.
   - rewrite* sel_fieldss_subst.
     rewrite* sel_fieldss_subst.
-  - erewrite <- numpaths_subst_typ. eauto.
 Qed.
 
-Lemma repl_typ_subst: forall n p q T U,
-  repl_typ n p q T U ->
+Lemma repl_typ_subst: forall p q T U,
+  repl_typ p q T U ->
   forall x y,
-  repl_typ n (subst_path x y p) (subst_path x y q) (subst_typ x y T) (subst_typ x y U).
+  repl_typ (subst_path x y p) (subst_path x y q) (subst_typ x y T) (subst_typ x y U).
 Proof.
   destruct repl_typ_subst_mutind; eauto.
 Qed.
